Q2 file namechange

SearchAddends.dfy
@@ -9,8 +9,129 @@ predicate HasAddends(q: seq<int>, x: int)
 }
 
 method FindAddends(q: seq<int>, x: int) returns (i: nat, j: nat)
-	requires Sorted(q) && HasAddends(q, x)
-	ensures i < j < |q| && q[i]+q[j] == x
+	requires Sorted(q)
+    requires HasAddends(q, x)
+	ensures 0 <= i < j < |q| && q[i]+q[j] == x
+{
+    // Introduce logical constants
+        ghost var i_result, j_result :|
+            0 <= i_result < j_result < |q|
+            && q[i_result] + q[j_result] == x;
+
+    i, j := FindAddends_WithLogicalConstants(q, x, i_result, j_result);
+}
+
+method {:verify false} FindAddends_WithLogicalConstants(q: seq<int>, x: int, ghost i_result : nat, ghost j_result:nat) returns(i: nat, j:nat)
+requires Sorted(q)
+requires 0 <= i_result < j_result < |q|
+requires q[i_result] + q[j_result] == x
+ensures 0 <= i < j < |q|
+ensures q[i] + q[j] == x
+{
+    // Sequential composition
+    i, j := Init(q, x, i_result, j_result);
+    Lemma_init(q, x, i, j, i_result, j_result);
+    i, j := Iterate(q, x, i, j, i_result, j_result);
+}
+
+method {:verify true} Init(q: seq<int>, x : int, ghost i_result:nat, ghost j_result:nat ) returns (i:nat, j:nat)
+requires 0 <= i_result < j_result < |q|
+requires HasAddends(q, x)
+requires Sorted(q)
+ensures  0 <= i <= j < |q|
+ensures i <= i_result
+ensures j_result <= j
+{
+    i, j := 0, |q| - 1;
+}
+
+lemma Lemma_init(q: seq<int>, x : int, i : nat, j:nat, i_result:nat, j_result:nat )
+requires Sorted(q)
+requires 0 <= i_result < j_result < |q|
+requires  0 <= i <= j < |q|
+requires q[i_result] + q[j_result] == x
+requires i <= i_result
+requires j_result <= j
+ensures Inv(q, x, i, j, i_result, j_result)
+{
+
+}
+
+method {:verify true} Iterate (q: seq<int>,x: int, i0:nat , j0 :nat, ghost i_result:nat, ghost j_result:nat ) returns (i:nat, j:nat)
+requires Inv(q, x, i0, j0, i_result, j_result)
+ensures Inv(q, x, i, j, i_result, j_result)
+ensures q[i] + q[j] == x
+{
+    i, j := i0, j0;
+    while q[i] + q[j] != x
+        invariant Inv(q, x,i, j, i_result, j_result)
+        decreases j - i
+        {
+            i, j := LoopBody(q, x, i, j, i_result, j_result);
+        }
+}
+method {:verify true} LoopBody(q: seq<int>, x : int, i0 : nat, j0: nat, ghost i_result:nat, ghost j_result:nat) returns (i : nat, j:nat)
+requires Inv(q, x, i0, j0, i_result, j_result)
+requires q[i0] + q[j0] != x
+ensures Inv(q, x, i, j, i_result, j_result)
+ensures (j0 - i0) > (j - i)
+{
+    if (q[i0] + q[j0] < x)
+    {
+        i, j := IncI(q, x, i0, j0, i_result, j_result);
+    }
+    else // q[i0] + q[j0] > x
+    {
+        i, j := DecJ(q, x, i0, j0, i_result, j_result);
+    }
+
+}
+
+method {:verify true} IncI(q: seq<int>, x : int, i0 : nat, j0: nat, ghost i_result:nat, ghost j_result:nat) returns (i : nat, j:nat)
+requires Inv(q, x, i0, j0, i_result, j_result)
+requires q[i0] + q[j0] < x
+ensures Inv(q,x, i, j, i_result, j_result)
+ensures (j0 - i0) > (j - i)
+{
+    IncI_Lemma(q, x, i0, j0, i_result, j_result);
+    i, j := i0 + 1, j0;
+}
+
+method {:verify true} DecJ(q: seq<int>, x : int, i0 : nat, j0: nat, ghost i_result:nat, ghost j_result:nat) returns (i : nat, j:nat)
+requires Inv(q, x, i0, j0, i_result, j_result)
+requires q[i0] + q[j0] > x
+ensures Inv(q, x, i, j, i_result, j_result)
+ensures (j0 - i0) > (j - i)
+{
+    DecJ_Lemma(q, x, i0, j0, i_result, j_result);
+    i, j := i0, j0 - 1;
+}
+
+lemma DecJ_Lemma(q: seq<int>, x : int, i0 : nat, j0: nat, i_result:nat, j_result:nat)
+requires Inv(q, x, i0, j0, i_result, j_result)
+requires q[i0] + q[j0] > x
+ensures j0 - 1 >= j_result
+{
+
+}
+
+lemma IncI_Lemma (q: seq<int>, x : int, i0 : nat, j0: nat, i_result:nat, j_result:nat)
+requires Inv(q, x, i0, j0, i_result, j_result)
+requires q[i0] + q[j0] < x
+ensures i0 + 1 <= i_result
+{
+
+}
+
+predicate Inv(q:seq<int>, x:int, i:nat, j:nat, i_result:nat, j_result:nat)
+{
+    Sorted(q) 
+    && 0 <= i_result < j_result < |q|
+    && q[i_result] + q[j_result] == x
+    && 0 <= i <= j < |q|
+    && i <= i_result
+    && j_result <= j
+}
 
 method Main()
 {
